smc-next/DiffieHellman.ec
@@ -1,8 +1,10 @@
-(* UCCoreDiffieHellman.ec *)
+(* CoreDiffieHellman.ec *)
 
 prover quorum=2 ["Alt-Ergo" "Z3"].
 
 require import AllCore Distr.
+
+require import KeysExponentsAndPlainTexts.
 
 (********************** Keys, Exponents and Plain texts ***********************)
 
