uc-dsl/prelude/UCEncoding.ec
@@ -2,6 +2,8 @@
 
 (* Encoding and Partial Decoding Pairs *)
 
+prover [""].  (* no use of SMT provers *)
+
 require import AllCore.
 
 (* encoding/partial decoding pair (EPDP) *)
@@ -33,9 +35,6 @@ move : dec_y_bad.
 by rewrite -enc_x_eq_y valid_epdp_1.
 qed.
 
-op is_valid (epdp : ('a, 'b) epdp, y : 'b) : bool =
-  epdp.`dec y <> None.
-
 lemma epdp_intro (epdp : ('a, 'b) epdp) :
   (forall (x : 'a), epdp.`dec (epdp.`enc x) = Some x) =>
   (forall (y : 'b, x : 'a), epdp.`dec y = Some x => epdp.`enc x = y) =>
@@ -43,6 +42,11 @@ lemma epdp_intro (epdp : ('a, 'b) epdp) :
 proof.
 trivial.
 qed.
+
+(* is_valid epdp y checks whether y decodes in epdp *)
+
+op is_valid (epdp : ('a, 'b) epdp, y : 'b) : bool =
+  epdp.`dec y <> None.
 
 lemma is_valid_enc (epdp : ('a, 'b) epdp, x : 'a) :
   valid_epdp epdp => is_valid epdp (epdp.`enc x).
@@ -64,4 +68,58 @@ proof.
 rewrite /valid_epdp => [[_ dec_enc]].
 move => dec_some.
 by rewrite (dec_enc y).
+qed.
+
+(* identity EPDP *)
+
+op nosmt epdp_id : ('a, 'a) epdp =
+  {|enc = fun x => x; dec = fun y => Some y|}.
+
+lemma valid_epdp_id : valid_epdp epdp_id<:'a>.
+proof.
+rewrite /valid_epdp /epdp_id /= => y x -> //.
+qed.
+
+(* EPDP built from a bijection *)
+
+op nosmt epdp_bijection (f : 'a -> 'b, g : 'b -> 'a) : ('a, 'b) epdp =
+  {|enc = f; dec = (\o) Some g|}.
+
+lemma valid_epdp_bijection (f : 'a -> 'b, g : 'b -> 'a) :
+  cancel f g => cancel g f => valid_epdp (epdp_bijection f g).
+proof.
+move => cancel_fg cancel_gf.
+rewrite /valid_epdp /epdp_bijection /=.
+split => [x | y x].
+rewrite /(\o).
+congr; apply cancel_fg.
+rewrite /(\o) => /= <-.
+apply cancel_gf.
+qed.
+
+(* composition of EPDPs *)
+
+op nosmt epdp_comp
+     (epdp2 : ('b, 'c) epdp) (epdp1 : ('a, 'b) epdp) : ('a, 'c) epdp =
+  {|enc = (\o) epdp2.`enc epdp1.`enc;
+    dec =
+      fun z =>
+        match epdp2.`dec z with
+        | None   => None
+        | Some y => epdp1.`dec y
+        end|}.
+
+lemma valid_epdp_comp (epdp2 : ('b, 'c) epdp) (epdp1 : ('a, 'b) epdp) :
+  valid_epdp epdp2 => valid_epdp epdp1 =>
+  valid_epdp (epdp_comp epdp2 epdp1).
+proof.
+move => valid2 valid1.
+rewrite /valid_epdp /epdp_comp /(\o) /=.
+split => [x | y x match_eq_some].
+by rewrite epdp_enc_dec //= epdp_enc_dec.
+have val_y : epdp2.`dec y = Some (epdp1.`enc x).
+  move : match_eq_some.
+  case (epdp2.`dec y) => //= x0 val_x0.
+  rewrite (epdp_dec_enc _ _ x0) //.
+by rewrite (epdp_dec_enc _ _ y).
 qed.
